leetcode/InvertTreeDev.dfy
@@ -1,6 +1,8 @@
 include "./invertTree.dfy"
+include "./preorderTraversalDefs.dfy"
 module InvertTreeDev {
     import opened InvertBinaryTree 
+    import opened PreorderTraversalSupp
 
     // lemma {:verify } {:vcs_split_on_every_assert} PreorderTraversalSubSlices2(root: TreeNode)
     //     requires root.Valid()
@@ -184,4 +186,117 @@ module InvertTreeDev {
             assert false;
         }
     }
+
+    lemma PreorderTraversal2SubSlices(root: TreeNode, node: TreeNode) returns (k: nat)
+        requires root.Valid()
+        requires node.Valid()
+        requires node in root.repr
+        ensures 0<=k < |PreorderTraversal2(root)|
+        ensures |PreorderTraversal2(node)|+k <= |PreorderTraversal2(root)| 
+        ensures PreorderTraversal2(node) == PreorderTraversal2(root)[k..|PreorderTraversal2(node)|+k]
+        decreases root.repr
+    {
+        TheyAreEqual(root);
+        TheyAreEqual(node);
+        assert |PreorderTraversal(root)| == |PreorderTraversal2(root)|;
+        k := PreorderTraversalSubSlices2(root, node);
+    }
+    // ghost predicate AllDisjoint(ts: seq<TreeNode>)
+    //     reads set x | 0 <= x < |ts| :: ts[x]
+    // {
+    //     forall x, y :: 0 <= x < y < |ts| && x != y ==> ts[x].repr !! ts[y].repr
+    // }
+    // lemma  AllDisjointMaint(stack: seq<TreeNode>, current: TreeNode)
+    //     requires |stack| > 0
+    //     requires AllDisjoint(stack)
+    //     requires forall x :: x in stack ==> x.Valid()
+    //     requires current == stack[|stack|-1]
+    //     ensures current.left != null && current.right != null ==> AllDisjoint(stack[..|stack|-1]+[current.right, current.left])
+    //     ensures current.left != null && current.right == null ==> AllDisjoint(stack[..|stack|-1]+[current.left])
+    //     ensures current.left == null && current.right != null ==> AllDisjoint(stack[..|stack|-1]+[current.right])
+    //     ensures current.left == null && current.right == null ==> AllDisjoint(stack[..|stack|-1])
+    // {
+    //         assert current.Valid();
+    //         if current.right != null && current.left != null {
+    //             // assert AllDisjoint(stack[..|stack|-1]+[current.right, current.left]);
+    //         } else if current.right != null && current.left == null {
+    //             assert current.right.repr < current.repr;
+    //             // assert AllDisjoint(stack[..|stack|-1]+[current.right]);
+    //         } else if current.right == null && current.left != null {
+    //             // assert AllDisjoint(stack[..|stack|-1]+[current.left]);
+    //         }else {
+    //             // assert AllDisjoint(stack[..|stack|-1]);
+    //         }
+    // }
+    // ghost function TreeUnion(nodes: seq<TreeNode>): set<TreeNode>
+    //     reads set x | 0 <= x < |nodes| :: nodes[x]
+    // {
+    // if |nodes| > 0 then nodes[0].repr + TreeUnion(nodes[1..]) else {}
+    // }
+
+    method {:isolate_assertions } TraverseBasic(root: TreeNode) returns (result: seq<TreeNode>)
+        requires root.Valid()
+        ensures result == PreorderTraversal2(root)
+    {
+        traversalSize(root);
+        TheyAreEqual(root);
+        var stack := [root];
+        var i := 0;
+        var unvisited: set<TreeNode> := root.repr;
+        var visited: set<TreeNode> := {};
+        result := [];
+        while |stack| > 0 
+            invariant forall x :: x in stack ==> x in root.repr
+            invariant forall x :: x in stack ==> x != null && x.Valid()
+            invariant AllDisjoint(stack)
+            invariant unvisited == TreeUnion(stack)
+            invariant unvisited !! visited
+            /*verifies */
+            invariant unvisited + visited == root.repr
+            invariant i == |result|
+            invariant i == |visited|
+            invariant i <= |root.repr|
+            invariant result == PreorderTraversal2(root)[0..i]
+            decreases |root.repr| - i
+        {
+            var current := stack[|stack|-1];
+            // TreeUnionLemma2(stack, root, current);
+            assert stack == stack[0..|stack|-1] + [current];
+            TreeUnionConcat(stack[0..|stack|-1] , [current]);
+            assert current in TreeUnion(stack);
+            assert current !in visited;
+            //The following was extracted into the function childStack();
+            ChildNodesAreValid(root, current);
+            AllDisjointMaint(stack, current);
+            TreeUnionMaint(stack, current, unvisited);
+            var stack' := childStack(current);
+
+            stack := stack[..|stack|-1]+stack';
+            result := result + [current];
+            visited := visited + {current};
+            unvisited := unvisited-{current};
+
+            i := i + 1;
+        }
+
+        assert i == |root.repr|;
+        assert i == |PreorderTraversal2(root)|;
+        assert PreorderTraversal2(root) == PreorderTraversal2(root)[0..i];
+        return result;
+    }
+    // lemma {:verify } PreorderTraversalSubSlices(root: TreeNode)
+    //     requires root.Valid()
+    //     requires forall node :: node in root.repr ==> node.Valid()
+    //     ensures forall node :: node in root.repr ==> exists k :: 0<=k < |PreorderTraversal(root)| && |PreorderTraversal(node)|+k <= |PreorderTraversal(root)| && PreorderTraversal(node) == PreorderTraversal(root)[k..|PreorderTraversal(node)|+k]
+    //     decreases root.repr
+    // {
+    //     forall node | node in root.repr 
+    //         ensures exists k {:trigger PreorderTraversal(node)}:: 0<=k < |PreorderTraversal(root)| && |PreorderTraversal(node)|+k <= |PreorderTraversal(root)| && PreorderTraversal(node) == PreorderTraversal(root)[k..|PreorderTraversal(node)|+k]
+    //     {
+    //         var x := PreorderTraversalSubSlices2(root, node);
+    //         assert 0<=x < |PreorderTraversal(root)|;
+    //         assert |PreorderTraversal(node)|+x <= |PreorderTraversal(root)|;
+    //         assert PreorderTraversal(node) == PreorderTraversal(root)[x..|PreorderTraversal(node)|+x];
+    //     }
+    // }
 }
